{
 "cells": [
  {
   "cell_type": "markdown",
   "id": "ccd95276-5b35-4f24-8071-07d48be4c403",
   "metadata": {},
   "source": [
    "<h1>\n",
    "    <center>\n",
    "        Math 104A Homework 6\n",
    "    </center>\n",
    "</h1>\n",
    "<h2>\n",
    "    <center>\n",
    "        Rad Mallari\n",
    "        <br>\n",
    "        8360828\n",
    "    </center>\n",
    "</h2><br><br>\n",
    "<b>1.)</b> Construct orthogonal polynomials of degree $0$, $1$, and $2$ on the interval $(0,1)$ with respect to the weight function:<br>\n",
    "&emsp;<b>a.)</b> $w(x)=\\log\\frac{1}{x}$<br>\n",
    "&emsp;<b>b.)</b> $w(x)=\\frac{1}{\\sqrt{x}}$<br>\n",
    "<b>Proof:</b><br>\n",
    "&emsp;<b>a.)</b> Letting $\\{g_{1},g_{2},...,g_{n}\\}$ be an orthonormal system in an inner-product space $E$, we can construct orthogonal polynomials $p_{0}(x),p_{1}(x),...,p_{n}(x)$ defined as:\n",
    "$$p_{n}(x)=(x-a_{n})p_{n-1}(x)-b_{n}p_{n-2}(x)\\quad(n\\geq 2)\\quad p_{0}(x)=1,\\quad p_{1}(x)=x-a_{1}$$\n",
    "&emsp; Where our unknowns are given by:\n",
    "$$a_{n}=\\frac{\\langle xp_{n-1}\\rangle, p_{n-1}\\rangle}{\\langle p_{n-1},p_{n-1}\\rangle}$$\n",
    "$$b_{n}=\\frac{\\langle xp_{n-1}\\rangle, p_{n-2}\\rangle}{\\langle p_{n-2},p_{n-2}\\rangle}$$\n",
    "$$\\langle f,g\\rangle=\\int_{a}^{b}f(x)g(x)w(x)dx$$\n",
    "&emsp; Therefore, we have that $p_{0}=1$, $p_{1}=x-a_{1}$, and $p_{2}=(x-a_{2})p_{1}(x)-b_{2}p_{0}(x)=(x-a_{2})(x-a_{1})-b_{2}$. Now solving for $a_{1},a_{2},b_{2}$:\n",
    "$$a_{1}=\\frac{\\langle x,1\\rangle}{\\langle 1,1\\rangle}=\\frac{\\int_{0}^{1}x\\log\\frac{1}{x}dx}{\\int_{0}^{1}\\log\\frac{1}{x}dx}=\\frac{\\frac{1}{4}}{1}=\\frac{1}{4}$$\n",
    "$$a_{2}=\\frac{\\langle x(x-\\frac{1}{4}),(x-\\frac{1}{4})\\rangle}{\\langle(x-\\frac{1}{4}),(x-\\frac{1}{4})\\rangle}=\\frac{\\int_{0}^{1}x\\left(x-\\frac{1}{4}\\right)^{2}\\log\\frac{1}{x}dx}{\\int_{0}^{1}\\left(x-\\frac{1}{4}\\right)^{2}\\log\\frac{1}{x}dx}=\\frac{\\frac{13}{576}}{\\frac{7}{144}}=\\frac{13}{28}$$\n",
    "$$b_{2}=\\frac{\\langle x(x-\\frac{1}{4}),1\\rangle}{\\langle1,1\\rangle}=\\frac{\\int_{0}^{1}\\left(x^{2}-\\frac{1}{4}x\\right)\\log\\frac{1}{x}dx}{\\int_{0}^{1}\\log\\frac{1}{x}dx}=\\frac{\\frac{7}{144}}{1}=\\frac{7}{144}$$\n",
    "&emsp; Altogether, for degree $0\\Rightarrow p_{0}(x)=1$, for degree $1\\Rightarrow p_{1}(x)=x-\\frac{1}{4}$, for degree $2\\Rightarrow p_{2}(x)=(x-\\frac{13}{28})(x-\\frac{1}{4})-\\frac{7}{144}$<br>\n",
    "&emsp;<b>b.)</b> Similarly, we find our $a_{1},a_{2},b_{2}$:\n",
    "$$a_{1}=\\frac{\\langle x,1\\rangle}{\\langle 1,1\\rangle}=\\frac{\\int_{0}^{1}x\\frac{1}{\\sqrt{x}}dx}{\\int_{0}^{1}\\frac{1}{\\sqrt{x}}dx}=\\frac{\\frac{2}{3}}{2}=\\frac{1}{3}$$\n",
    "$$a_{2}=\\frac{\\langle x\\left(x-\\frac{1}{3}\\right),\\left(x-\\frac{1}{3}\\right)\\rangle}{\\langle\\left(x-\\frac{1}{3}\\right),\\left(x-\\frac{1}{3}\\right)\\rangle}=\\frac{\\int_{0}^{1}x\\left(x-\\frac{1}{3}\\right)^{2}\\frac{1}{\\sqrt{x}}dx}{\\int_{0}^{1}{\\left(x-\\frac{1}{3}\\right)^{2}\\frac{1}{\\sqrt{x}}dx}}=\\frac{\\frac{88}{945}}{\\frac{8}{45}}=\\frac{11}{21}$$\n",
    "$$b_{2}=\\frac{\\langle x(x-\\frac{1}{3}),1\\rangle}{\\langle1,1\\rangle}=\\frac{\\int_{0}^{1}\\left(x^{2}-\\frac{1}{3}x\\right)\\frac{1}{\\sqrt{x}}dx}{\\int_{0}^{1}\\frac{1}{\\sqrt{x}}dx}=\\frac{\\frac{8}{45}}{2}=\\frac{4}{45}$$\n",
    "&emsp; So we conclude with $p_{0}(x)=1$, $p_{1}(x)=x-\\frac{1}{3}$, $p_{2}(x)=\\left(x-\\frac{11}{21}\\right)\\left(x-\\frac{1}{3}\\right)-\\frac{4}{45}$<br>\n",
    "<br>\n",
    "<b>2.)</b> In each of the following, find the least square approximation of degrees $0$, $1$, and $2$ for the function $f(x)=\\sin(x)$ on the interval $(a,b)$ with respect to the weight function $w(x)=1$.<br>\n",
    "&emsp;<b>a.)</b> $(a,b)$ = $(-\\pi,\\pi)$<br>\n",
    "&emsp;<b>b.)</b> $(a,b)$ = $(-\\frac{\\pi}{2},\\frac{\\pi}{2})$<br>\n",
    "<b>Proof:</b><br>\n",
    "&emsp;<b>a.)</b> Similar to <b>Homework 5, Problem 6</b>, we use:\n",
    "$$E(a_{0},a_{1},...,a_{n})=\\sum_{j=1}^{m}(y_{i}-\\sum_{k=0}^{n}a_{k}x_{i}^{k})^{2}$$\n",
    "&emsp; Then for degree $0$, we have the following:\n",
    "$$E(a_{0})=\\int_{-\\pi}^{\\pi}(\\sin(x)-a_{0})^{2}\\Rightarrow \\frac{\\partial E}{a_{0}}=2\\int_{-\\pi}^{\\pi}(\\sin(x)-a_{0})dx=0$$\n",
    "$$\\Rightarrow (-\\cos(x)-a_{0}x)\\bigg|_{-\\pi}^{\\pi}=0$$\n",
    "$$\\Rightarrow (-\\cos(\\pi)-a_{0}\\pi)-(\\cos(-\\pi)+a_{0}\\pi)=0$$\n",
    "$$\\Rightarrow 2a_{0}\\pi=0\\Rightarrow a_{0}=0$$\n",
    "&emsp; So for degree $0$, $p_{0}(x)=0$<br>\n",
    "&emsp; For degree $1$, we have:\n",
    "$$E(a_{0},a_{1})=\\int_{-\\pi}^{\\pi}(\\sin(x)-(a_{0}+a_{1}))^{2}$$\n",
    "&emsp; Solving for $a_{0}$:\n",
    "$$\\frac{\\partial E}{\\partial a_{0}}=-2\\int_{-\\pi}^{\\pi}(\\sin(x)-a_{0}-a_{1}x)dx=0$$\n",
    "$$\\Rightarrow (-\\cos(x)-a_{0}x-\\frac{1}{2}a_{1}x^{2})\\bigg|_{-\\pi}^{\\pi}=0$$\n",
    "$$\\Rightarrow (1-a_{0}\\pi-\\frac{1}{2}a_{1}\\pi^{2})-(1+a_{0}\\pi-\\frac{1}{2}a_{1}\\pi^{2})=0$$\n",
    "$$\\Rightarrow -2a_{0}\\pi=0\\Rightarrow a_{0}=0$$\n",
    "&emsp; Then for $a_{1}$:\n",
    "$$\\frac{\\partial E}{\\partial a_{1}}=-2\\int_{-\\pi}^{\\pi}(\\sin(x)-a_{0}-a_{1}x)(x)dx=0$$\n",
    "$$\\Rightarrow \\int_{-\\pi}^{\\pi}x\\sin(x)dx-\\int_{-\\pi}^{\\pi}a_{0}xdx-\\int_{-\\pi}^{\\pi}a_{1}x^{2}dx=0$$\n",
    "$$\\Rightarrow (\\sin(x)-x\\cos(x))\\bigg|_{\\pi}^{0}-\\frac{1}{2}a_{0}x^{2}\\bigg|_{\\pi}^{0}-\\frac{1}{3}a_{1}x^{3}\\bigg|_{\\pi}^{0}=0$$\n",
    "$$\\Rightarrow 2\\pi-0-\\frac{2\\pi^{3}}{9}a_{1}=0\\Rightarrow a_{1}=\\frac{9}{\\pi^{2}}$$\n",
    "&emsp; Therefore, for degree $1$, $p_{0}(x)=\\frac{9}{\\pi^{2}}x$<br>\n",
    "&emsp; Then, for degree $2$:\n",
    "$$E(a_{0},a_{1},a_{2})=\\int_{-\\pi}^{\\pi}(\\sin(x)-a_{0}-a_{1}x-a_{2}x^{2})dx=0$$\n",
    "&emsp; For one equation,\n",
    "$$\\frac{\\partial E}{\\partial a_{0}}=-2\\int_{-\\pi}^{\\pi}(\\sin(x)-a_{0}-a_{1}x-a_{2}x^{2})dx=0$$\n",
    "$$\\Rightarrow (-\\cos(x)-a_{0}x-\\frac{1}{2}a_{1}x^{2}-\\frac{1}{3}x^{3})\\bigg|_{-\\pi}^{\\pi}=0$$\n",
    "$$\\Rightarrow -2\\pi a_{0}-\\frac{2}{3}\\pi^{3}a_{2}=0\\Rightarrow a_{0}=\\frac{1}{3}a_{2}$$\n",
    "&emsp; Then the next,\n",
    "$$\\frac{\\partial E}{\\partial a_{1}}=-2\\int_{-\\pi}^{\\pi}(\\sin(x)-a_{0}-a_{1}x-a_{2}x^{2})(x)dx=0$$\n",
    "$$\\Rightarrow \\int_{-\\pi}^{\\pi}(x\\sin(x)-a_{0}x-a_{1}x^{2}-a_{2}x^{3})dx=0$$\n",
    "$$\\Rightarrow (\\sin(x)-x\\cos(x)-\\frac{1}{2}a_{0}x^{2}-\\frac{1}{3}a_{1}x^{3}-\\frac{1}{4}a_{2}x^{4})\\bigg|_{-\\pi}^{\\pi}=0$$\n",
    "$$\\Rightarrow 2\\pi-\\frac{2}{3}a_{1}\\pi^{3}=0\\Rightarrow a_{1}=\\frac{3}{\\pi^{3}}$$\n",
    "&emsp; Finally,\n",
    "$$\\frac{\\partial E}{\\partial a_{2}}=-2\\int_{-\\pi}^{\\pi}(\\sin(x)-a_{0}-a_{1}x-a_{2}x^{2})(x^{2})dx=0$$\n",
    "$$\\Rightarrow \\int_{-\\pi}^{\\pi}(x^{2}\\sin(x)-a_{0}x^{2}-a_{1}x^{3}-a_{2}x^{4})dx=0$$\n",
    "$$\\Rightarrow (2x\\sin(x)+(2-x^{2})\\cos(x)-\\frac{1}{3}a_{0}x^{3}-\\frac{1}{4}a_{1}x^{4}-\\frac{1}{5}a_{2}x^{5})\\bigg|_{-\\pi}^{\\pi}=0$$\n",
    "$$\\Rightarrow -\\frac{2}{3}\\pi^{3}a_{0}-\\frac{2}{5}\\pi^{5}a_{2}=0\\Rightarrow a_{0}=\\frac{3}{5}\\pi^{2}a_{2}$$\n",
    "&emsp; Therefore, the system of equations gives us that $a_{0}=0$, $a_{1}=\\frac{3}{\\pi^{3}}$, $a_{2}=0$. So for degree $2$, $p_{2}=\\frac{3}{\\pi^{3}}x$<br>\n",
    "&emsp; <b>b.)</b> Again, for degree $0$,\n",
    "$$E(a_{0})=\\int_{\\frac{-\\pi}{2}}^{\\frac{\\pi}{2}}(\\sin(x)-a_{0})^{2}\\Rightarrow \\frac{\\partial E}{a_{0}}=2\\int_{\\frac{-\\pi}{2}}^{\\frac{\\pi}{2}}(\\sin(x)-a_{0})dx=0$$\n",
    "$$\\Rightarrow (-\\cos(x)-a_{0}x)\\bigg|_{\\frac{-\\pi}{2}}^{\\frac{\\pi}{2}}=0\\Rightarrow -\\pi a_{0}=0\\Rightarrow a_{0}=0$$\n",
    "&emsp; So, $p_{0}(x)=0$.<br>\n",
    "&emsp; For degree $1$:\n",
    "$$E(a_{0},a_{1})=\\int_{-\\pi}^{\\pi}(\\sin(x)-(a_{0}+a_{1}))^{2}$$\n",
    "$$\\Rightarrow \\frac{\\partial E}{\\partial a_{0}}=-2\\int_{\\frac{-\\pi}{2}}^{\\frac{\\pi}{2}}(\\sin(x)-a_{0}-a_{1}x)dx=0$$\n",
    "$$\\Rightarrow (x\\sin(x)-a_{0}x-\\frac{1}{2}a_{1}x^{2})\\bigg|_{-\\frac{\\pi}{2}}^{\\frac{\\pi}{2}}=0$$\n",
    "$$\\Rightarrow \\pi a_{0}=0\\Rightarrow a_{0}=0$$\n",
    "$$\\frac{\\partial E}{\\partial a_{1}}=-2\\int_{-\\frac{\\pi}{2}}^{\\frac{\\pi}{2}}(\\sin(x)-a_{0}-a_{1}x)(x)dx=0$$\n",
    "$$\\Rightarrow \\int_{-\\frac{\\pi}{2}}^{\\frac{\\pi}{2}}(x\\sin(x)-a_{0}x-a_{1}x^{2}-a_{2}x^{3})dx=0$$\n",
    "$$\\Rightarrow (\\sin(x)-x\\cos(x)-\\frac{1}{2}a_{0}x^{2}-\\frac{1}{3}a_{1}x^{3})\\bigg|_{-\\frac{\\pi}{2}}^{\\frac{\\pi}{2}}=0$$\n",
    "$$\\Rightarrow 2-\\frac{\\pi^{3}}{12}a_{1}=0\\Rightarrow a_{1}=\\frac{6}{\\pi^{3}}$$\n",
    "&emsp; Therefore, $p_{1}=\\frac{6}{\\pi^{3}}x$.<br>\n",
    "&emsp; Lastly, for degree $2$:\n",
    "$$E(a_{0},a_{1},a_{2})=\\int_{-\\frac{\\pi}{2}}^{\\frac{\\pi}{2}}(\\sin(x)-a_{0}-a_{1}x-a_{2}x^{2})dx=0$$\n",
    "$$\\frac{\\partial E}{\\partial a_{0}}=-2\\int_{-\\frac{\\pi}{2}}^{\\frac{\\pi}{2}}(\\sin(x)-a_{0}-a_{1}x-a_{2}x^{2})dx=0$$\n",
    "$$\\Rightarrow (-\\cos(x)-a_{0}x-\\frac{1}{2}a_{1}x^{2}-\\frac{1}{3}x^{3})\\bigg|_{-\\frac{\\pi}{2}}^{\\frac{\\pi}{2}}=0$$\n",
    "$$\\Rightarrow -\\frac{1}{2}\\pi a_{0}-\\frac{1}{12}\\pi^{3}a_{1}\\Rightarrow a_{0}=\\frac{1}{6}a_{1}$$\n",
    "$$\\frac{\\partial E}{\\partial a_{1}}=-2\\int_{-\\frac{\\pi}{2}}^{\\frac{\\pi}{2}}(\\sin(x)-a_{0}-a_{1}x-a_{2}x^{2})(x)dx=0$$\n",
    "$$\\Rightarrow \\int_{-\\frac{\\pi}{2}}^{\\frac{\\pi}{2}}(x\\sin(x)-a_{0}x-a_{1}x^{2}-a_{2}x^{3})dx=0$$\n",
    "$$\\Rightarrow (\\sin(x)-x\\cos(x)-\\frac{1}{2}a_{0}x^{2}-\\frac{1}{3}a_{1}x^{3}-\\frac{1}{4}a_{2}x^{4})\\bigg|_{-\\frac{\\pi}{2}}^{\\frac{\\pi}{2}}=0$$\n",
    "$$\\Rightarrow 2-\\frac{1}{12}a_{1}\\pi^{3}=0\\Rightarrow a_{1}=\\frac{24}{\\pi^{3}}$$\n",
    "$$\\frac{\\partial E}{\\partial a_{2}}=-2\\int_{-\\frac{\\pi}{2}}^{\\frac{\\pi}{2}}(\\sin(x)-a_{0}-a_{1}x-a_{2}x^{2})(x^{2})dx=0$$\n",
    "$$\\Rightarrow \\int_{-\\frac{\\pi}{2}}^{\\frac{\\pi}{2}}(x^{2}\\sin(x)-a_{0}x^{2}-a_{1}x^{3}-a_{2}x^{4})dx=0$$\n",
    "$$\\Rightarrow (2x\\sin(x)+(2-x^{2})\\cos(x)-\\frac{1}{3}a_{0}x^{3}-\\frac{1}{4}a_{1}x^{4}-\\frac{1}{5}a_{2}x^{5})\\bigg|_{-\\frac{\\pi}{2}}^{\\frac{\\pi}{2}}=0$$\n",
    "$$\\Rightarrow -\\frac{1}{12}\\pi^{3}a_{0}-\\frac{1}{80}\\pi^{5}a_{2}=0\\Rightarrow a_{0}=\\frac{1}{20}\\pi^{2}a_{2}$$\n",
    "&emsp; We conclude, $p_{2}=\\frac{24}{\\pi^{3}}x$<br>\n",
    "<b>3.)</b> Let $x_{0},x_{1},...,x_{n}$ be distinct points in $[a,b]$ and we interpolate a function $f(x)$ by a polynomial $p_{n}(x)$ by Lagrange interpolation method. Let $\\{l_{j}(x)^{(n)}\\}_{j=0}^{n}$ be the Lagrange polynomials used in Lagrange interpolation. Prove $\\sum_{j=0}^{n}l_{j}(x)^{(n)}=1$ for all $x$.<br>\n",
    "<b>Proof:</b><br>\n",
    "&emsp; We recall that $l_{j}(x)$ is defined as:\n",
    "$$l_{j}(x)=\\prod_{j=0, j\\neq i}^{n}\\frac{x-x_{j}}{x_{i}-x_{j}}\\quad(0\\leq i\\leq n)$$\n",
    "&emsp; And the Lagrange polynomial is:\n",
    "$$p(x)=\\sum_{j=0}^{n}y_{j}l_{j}(x)$$\n",
    "&emsp; Suppose we interpolate the function $y(x)=1$, then $1=\\sum_{j=1}^{n}(1)l_{j}(x)=y(x)$, thereby showing what we want and interpolating our function perfectly. Furthermore, since $p(x)$ is unique, it must always be the case that $\\sum_{j=0}^{n}l_{j}(x)=1$ for all $x$.<br>\n",
    "<b>4.)</b> Let $x_{0},x_{1},...,x_{n}$ be distinct points in $[a,b]$. Show that if $f$ and its first derivatives are defined respectively at points $x_{0},x_{1},...,x_{n}$, then there <b>exists a unique</b> polynomial $q$ of degree at most $2n+1$ such that\n",
    "$$q(x_{j})=f(x_{j}),\\quad\\textrm{and}\\quad q'(x_{j})=f'(x_{j})$$\n",
    "&emsp; for $j=0,1,...,n$.<br>\n",
    "<b>Proof:</b><br>\n",
    "&emsp; Assume there exists a different polynomial $t(x)$ where $\\textrm{Deg}(t(x))\\leq 2n+1$ such that\n",
    "$$t(x_{j})=f(x_{j}),\\quad\\textrm{and}\\quad t'(x_{j})=f'(x_{j})$$\n",
    "&emsp; for $j=0,1,...,n$. Then the polynomial $r(x)=t(x)-q(x)=0$ and $r'(x)=t'(x)-q'(x)=0$ is a polynomial of degree $2n+1$ with roots of multiplicity $2$ of $x_{0},x_{1},...,x_{n}$. To prove uniqueness, we let $s(x)$ be some polynomial, and $r(x)=s(x)(x-x_{0})^2(x-x_{1})^{2}...(x-x_{n})^{2}$. Then $s(x)$ must be $0$ since $r(x)$ should have $n$ zeros by the Fundamental Theorem of Algebra. If it is the case that $s(x)\\neq 0$, then $\\textrm{Deg}(r(x))>2n+1$ and $r(x)=0$. If $r(x)=0$, it is implied that $q(x)=t(x)$ therefore, $q(x)$ is unique."
   ]
  },
  {
   "cell_type": "code",
   "execution_count": null,
   "id": "9d43bd01-1fd9-42cc-8e7c-6f901c22ce93",
   "metadata": {},
   "outputs": [],
   "source": []
  }
 ],
 "metadata": {
  "kernelspec": {
   "display_name": "Python 3 (ipykernel)",
   "language": "python",
   "name": "python3"
  },
  "language_info": {
   "codemirror_mode": {
    "name": "ipython",
    "version": 3
   },
   "file_extension": ".py",
   "mimetype": "text/x-python",
   "name": "python",
   "nbconvert_exporter": "python",
   "pygments_lexer": "ipython3",
   "version": "3.9.10"
  }
 },
 "nbformat": 4,
 "nbformat_minor": 5
}
